Forest.v
@@ -1,0 +1,131 @@
+Require Export Graph.
+
+Require Export Path.
+(*TODO: maybe extend graph instead of providing function*)
+
+Module Type Forest(O: UsualOrderedType)(S Sg: FSetInterface.Sfun O)(G: Graph O Sg).
+
+  Module P := (Path.PathTheories O Sg G).
+
+  Parameter forest : Type.
+
+  Definition vertex := O.t.
+  
+  Parameter empty : forest.
+
+  Parameter is_empty: forest -> bool.
+
+  Parameter add_root: forest -> vertex -> forest.
+
+  Parameter contains_vertex: forest -> vertex -> bool.
+
+  Parameter add_child : forest -> vertex -> vertex -> forest.
+
+  Parameter is_child: forest -> vertex -> vertex -> bool.
+
+  (*Parameter get_children: forest -> vertex -> option (list vertex).*)
+
+  Parameter forest_to_graph: forest -> G.graph.
+
+  Parameter is_descendent: forest -> vertex -> vertex -> bool.
+
+  Definition is_parent f u v := is_child f v u.
+
+  Definition is_ancestor f u v := is_descendent f v u.
+
+  (*Parameter equal: tree -> tree -> bool.*)
+
+  Parameter empty_1: is_empty empty = true.
+
+  Parameter empty_2: forall f,
+    is_empty f = true <-> (forall u, contains_vertex f u = false).
+
+  Parameter add_child_1: forall t u v,
+    contains_vertex t u = true ->
+    contains_vertex t v = false ->
+    is_child (add_child t u v) u v = true.
+
+  Parameter add_child_2: forall t u v a b,
+    is_child t u v = true ->
+    is_child (add_child t a b) u v = true.
+
+  Parameter add_child_3: forall t u v a,
+    contains_vertex t a = true ->
+    contains_vertex (add_child t u v) a = true.
+
+  Parameter add_child_4: forall t u v,
+    contains_vertex t v = true ->
+    is_child (add_child t u v) u v = false.
+
+  Parameter add_child_5: forall t u v,
+    contains_vertex t u = true ->
+    contains_vertex (add_child t u v) v = true.
+
+  Parameter add_child_6: forall t u v a,
+    contains_vertex (add_child t u v) a = true -> contains_vertex t a = true \/ a = v.
+
+  Parameter add_root_1: forall f u,
+    contains_vertex f u = false ->
+    contains_vertex (add_root f u) u = true.
+
+  Parameter add_root_2: forall f u v,
+    contains_vertex f v = true ->
+    contains_vertex (add_root f u) v = true.
+
+(*
+  Parameter singleton_1: forall v,
+    root (singleton v) = Some v.
+
+  Parameter singleton_2: forall v u,
+    contains_vertex (singleton v) u = true <-> u = v.*)
+
+  (*Parameter root_1: forall t u v r,
+    root t = Some r <->
+    root (add_child t u v) = Some r.
+
+  Parameter root_2: forall t,
+    root t = None <-> forall v, contains_vertex t v = false.*)
+
+  (*Parameter empty_1: forall v,
+    contains_vertex empty v = false.
+
+  Parameter empty_2: forall u v,
+    is_child empty u v = false.*)
+
+  (*Parameter add_child_3: forall t u v,
+    contains_vertex t v = true ->
+    equal (add_child t u v) t = true.*)
+
+
+
+  (*Parameter get_children_1: forall t u,
+    contains_vertex t u = true <->
+    exists l, get_children t u = Some l.
+
+  Parameter get_children_2: forall t u v l,
+    get_children t u = Some l ->
+    (is_child t u v = true <-> In v l).*)
+
+  Parameter tree_to_graph_1: forall t u,
+    contains_vertex t u = true <-> G.contains_vertex (forest_to_graph t) u = true.
+
+  Parameter tree_to_graph_2: forall t u v,
+    is_child t u v = true <-> G.contains_edge (forest_to_graph t) u v = true.
+
+  Parameter tree_to_graph_3: forall t,
+    P.acyclic (forest_to_graph t).
+
+  Parameter is_descendent_edge: forall t u v,
+    is_child t u v = true ->
+    is_descendent t u v = true.
+
+  Parameter is_descendent_trans: forall t u v w,
+    is_descendent t u v = true ->
+    is_descendent t v w = true ->
+    is_descendent t u w = true.
+    
+(*might need equal lemma to ensure it is acyclic but we will see*)
+End Forest.
+     
+     
+     
